- Some judgements in HsJudgement - State and prove Translation preserves Judgment soundness - FrameMetada and indexing function for surface level Context

Hs/HsJudgment.lean
@@ -1,2 +1,73 @@
 import Hs.HsTerm
 import Hs.HsCtx
+
+def pad_empty_ctx : Nat -> HsCtx HsTerm
+| 0 => [.empty]
+| n + 1 => .empty :: pad_empty_ctx n
+
+
+inductive JIdx where
+| CtxJ | TermJ | TypeJ | KindJ
+
+@[simp]
+abbrev JudgmentType : JIdx -> Type
+| .CtxJ => Unit
+| .TermJ => HsTerm × HsTerm
+| .KindJ => HsTerm × HsTerm
+| .TypeJ => HsTerm × HsTerm
+
+inductive HsJudgment : (i : JIdx) -> HsCtx HsTerm -> JudgmentType i -> Prop where
+| wfnil : HsJudgment .CtxJ [] ()
+| wfempty :
+  HsJudgment .CtxJ Γ () ->
+  HsJudgment .CtxJ (.empty :: Γ) ()
+| wfkind :
+  HsJudgment .CtxJ Γ  () ->
+  HsJudgment .TermJ Γ (k, `□) ->
+  HsJudgment .CtxJ (.kind k ::  Γ) ()
+| wftype :
+  HsJudgment .CtxJ Γ () ->
+  HsJudgment .TermJ Γ (A, `★) ->
+  HsJudgment .CtxJ (.type A :: Γ) ()
+| wfdatatypeDecl :
+  HsJudgment .CtxJ Γ () ->
+  HsJudgment .TermJ Γ (k, `□) ->
+  ∀ p: i < ctors.length, HsJudgment .TermJ (pad_empty_ctx i ++ Γ) (ctors[i]'(by assumption), `★) ->
+  HsJudgment .CtxJ (.datatypeDecl k ctors :: Γ) ()
+| wfterm :
+  HsJudgment .CtxJ Γ () ->
+  HsJudgment .TermJ Γ (A, `★) ->
+  HsJudgment .TermJ Γ (t, A) ->
+  HsJudgment .CtxJ (.term A t :: Γ) ()
+
+
+| wfstar :
+  HsJudgment .CtxJ Γ () ->
+  HsJudgment .KindJ Γ (`★, `□)
+| wfkarrow :
+  HsJudgment .CtxJ Γ () ->
+  HsJudgment .KindJ Γ (κ1, `□) ->
+  HsJudgment .KindJ Γ (κ2, `□) ->
+  HsJudgment .KindJ Γ (κ1 `-k> κ2, `□)
+
+
+| varTy :
+  HsJudgment .CtxJ Γ () ->
+  FrameMetadata.get_type (Γ s@ x) = .some T ->
+  HsJudgment .TypeJ Γ (`#x, T)
+
+| arrowt :
+  HsJudgment .CtxJ Γ () ->
+  HsJudgment .TypeJ Γ (A, `★) ->
+  HsJudgment .TypeJ (.empty :: Γ) (B, `★) ->
+  HsJudgment .TypeJ Γ (A → B, `★)
+| allt :
+  HsJudgment .CtxJ Γ () ->
+  HsJudgment .TypeJ Γ (A, `★) ->
+  HsJudgment .TypeJ (.type A :: Γ) (B, `★) ->
+  HsJudgment .TypeJ Γ (`∀{A} B, `★)
+| appt :
+  HsJudgment .CtxJ Γ () ->
+  HsJudgment .TypeJ Γ (T, k `-k> k') ->
+  HsJudgment .TypeJ Γ (A, k) ->
+  HsJudgment .TypeJ Γ (T `•k A, `★)
